Updated and unified dynamic indices Updated some notation

Logic/DL/Syntax.lean
@@ -32,19 +32,4 @@ def disj (φ ψ: DLForm RelType AtomType) : DLForm RelType AtomType := imp (not 
 --box [α]φ
 def box (α: Relation RelType) (φ: DLForm RelType AtomType) : DLForm RelType AtomType := not (diamond α (not φ))
 
-
--- concrete relation type for dynamic indices
-inductive DynIdxSym: Type
-  | line: Nat → DynIdxSym
-  | dollar: DynIdxSym
-  | hash: DynIdxSym
-deriving DecidableEq, BEq
-
-abbrev DynIndex := List DynIdxSym
-
--- concrete formula type, strings for modelling assertions
-inductive Atoms: Type
-  | name: String → Atoms
-deriving DecidableEq, BEq
-
 end Logic.DL
