Logic/REPEAT/Semantics.lean
@@ -1,18 +1,19 @@
 import Mathlib.Data.Set.Basic
 import Logic.REPEAT.Syntax
 import Logic.DL.Semantics
+import Logic.Common.DynamicIndex
 
-namespace Logic.REPEAT
+namespace Logic.DL
 
 
-
+/-
 inductive DynIndex where
   | root : DynIndex
   | line : DynIndex → Nat → DynIndex
   | dollar: DynIndex → DynIndex
   | hash: DynIndex → DynIndex
 deriving DecidableEq
-
+-/
 /--
 Encapsulates a control flow trace, which is a triple P = (Q, prompt, tar) where
 * `Q` is a Set of States, represented as `Set DynIndex`
@@ -39,22 +40,28 @@ Partial stmt function, which evaluates to the statement at a given dynamic index
 def stmt (cft: CFTrace) (idx: DynIndex) : Option Stmt :=
   match idx with
     | .root => some cft.prompt -- stmt(ε) = prompt, where [] represents ε
-    | .line s i  => -- stmt(s i)
+    | .cons s sym  => -- stmt(s i)
+        match sym with
+          | .line i =>
+              match cft.tar s with  --cft.tar s is the current procedure
+                | none => none       --shouldn't occur in valid cft (i.e. s i ∈ Q → ∃ p, tar s = some p)
+                | some proc =>
+                    match proc.body.find? (λ ls => ls.line == i) with
+                      | none => none
+                      | some ls => some ls.stmt
 
-        match cft.tar s with --ctf.tar s is the current procedure
-          | none => none          --shouldn't occur in valid cft (i.e. s i ∈ Q → ∃ p, tar s = some p)
-          | some proc => --TODO: Why no list indices as line numbers?
-              match proc.body.find? (λ ls => ls.line == i) with --extract statement at line i
-                | none => none
-                | some ls => some ls.stmt
-    | _ => none
+          | _ => none
 
 
+def currentProcId (cft: CFTrace) (idx: DynIndex) : Option Int :=
+  match idx with
+    | .root =>     match cft.prompt with
+                    | Stmt.call (Expr.const id) _ => id   --TODO: Requires call to constant, i.e. no call arithmetic is possible => otherwise currentProcId depends on val
+                    | _ => none
+    | .cons s _ => match cft.tar s with
+                    | some proc => proc.id
+                    | none => none
 
---notation for readability
-notation "ε" => DynIndex.root
-notation:max s "$" => DynIndex.dollar s
-notation:max s "#" => DynIndex.hash s
 
 /- Closure properties for the set of states Q in a cft-/
 
@@ -63,50 +70,51 @@ def rootClosure (cft: CFTrace) : Prop :=
   ε ∈ cft.Q ∧
   ∃ expr args, cft.prompt = Stmt.call expr args
 
+
 -- if s ∈ Q and stmt (s) is a call `call expr args`, then s 0 ∈ Q and tar(s) maps to a arity matching procedure
 def callClosure (cft: CFTrace) : Prop :=
   ∀ s expr args,
     ((s ∈ cft.Q ∧ stmt cft s = some (Stmt.call expr args)) →
 
-      DynIndex.line s 0 ∈ cft.Q ∧
+      line s 0 ∈ cft.Q ∧
       ∃ proc, (cft.tar s = some proc ∧ args.length = proc.params.length))
 
 -- if s i ∈ Q and stmt(s i) is an assignment `v[e₀] = e₁`, then s (i+1) ∈ Q
 def assignClosure (cft: CFTrace) : Prop :=
   ∀ s i v e₀ e₁,
-    (DynIndex.line s i ∈ cft.Q ∧
-     stmt cft (DynIndex.line s i) = some (Stmt.assign v e₀ e₁) →
+    (line s i ∈ cft.Q ∧
+     stmt cft (line s i) = some (Stmt.assign v e₀ e₁) →
 
-     DynIndex.line s (i + 1) ∈ cft.Q)
+     line s (i + 1) ∈ cft.Q)
 
 -- if s i ∈ Q and stmt(s i) is a returnIf `if e return ` then either s (i+1) ∈ Q or s # ∈ Q
 def returnClosure (cft: CFTrace) : Prop :=
   ∀ s i e,
-    (DynIndex.line s i) ∈ cft.Q ∧
-     stmt cft (DynIndex.line s i) = some (Stmt.returnIf e) →
+    (line s i) ∈ cft.Q ∧
+     stmt cft (line s i) = some (Stmt.returnIf e) →
 
-     (DynIndex.line s (i + 1) ∈ cft.Q ∨ s # ∈ cft.Q)
+     (line s (i + 1) ∈ cft.Q ∨ s ∘ # ∈ cft.Q)
 
 -- if s i ∈ Q and stmt(s i) is `repeat`, then s $ ∈ Q, s $ 0 ∈ Q and tar(s $) = tar(s)
 def repeatClosure (cft: CFTrace) : Prop :=
   ∀ s i proc,
-    (DynIndex.line s i ∈ cft.Q ∧
-     stmt cft (DynIndex.line s i) = some (Stmt.repeat) ∧
+    (line s i ∈ cft.Q ∧
+     stmt cft (line s i) = some (Stmt.repeat) ∧
      cft.tar s = some proc) →
 
-      (s $ ∈ cft.Q ∧
-       DynIndex.line (s $) 0 ∈ cft.Q ∧
-       cft.tar (s $) = some proc)
+      (s ∘ $ ∈ cft.Q ∧
+       line (s ∘ $) 0 ∈ cft.Q ∧
+       cft.tar (s ∘ $) = some proc)
 
 -- if s $ # ∈ Q, then s # ∈ Q
 def repeatReturnClosure (cft: CFTrace) : Prop :=
   ∀ s,
-    (s $) # ∈ cft.Q → s # ∈ cft.Q
+    (s ∘ $) ∘ # ∈ cft.Q → s ∘ # ∈ cft.Q
 
 -- if s i # ∈ Q, then s (i + 1) ∈ Q
 def callReturnClosure (cft: CFTrace) : Prop :=
   ∀ s i,
-    (DynIndex.line s i) # ∈ cft.Q → DynIndex.line s (i +1) ∈ cft.Q
+    (line s i) ∘ # ∈ cft.Q → line s (i + 1) ∈ cft.Q
 
 
 /- No junk properties for the set of states Q in a cft -/
@@ -114,40 +122,40 @@ def callReturnClosure (cft: CFTrace) : Prop :=
 -- if s 0 ∈ Q, then s = ε or stmt(s) is a call `call expr args` with matching tar arity or s = t $ with stmt(t i) = `repeat`
 def noJunkCalls (cft: CFTrace) : Prop :=
   ∀ s,
-    DynIndex.line s 0 ∈ cft.Q →
+    line s 0 ∈ cft.Q →
       (s = ε ∨
        (∃ expr args proc, s ∈ cft.Q ∧ stmt cft s = some (Stmt.call expr args) ∧
         cft.tar s = some proc ∧ args.length = proc.params.length) ∨
-       (∃ t i, s = t $ ∧ DynIndex.line t i ∈ cft.Q ∧ stmt cft (DynIndex.line t i) = some (Stmt.repeat))
+       (∃ t i, s = t ∘ $ ∧ line t i ∈ cft.Q ∧ stmt cft (line t i) = some (Stmt.repeat))
        )
 
 -- if s i+1 ∈ Q, then s i ∈ Q and stmt(s i) is an assign `v[e₀] = e₁` or returnIf `if e return`
 def noJunkLines (cft: CFTrace) : Prop :=
   ∀ s i,
-    DynIndex.line s (i+1) ∈ cft.Q →
+    line s (i+1) ∈ cft.Q →
       ((∃ v e₀ e₁,
-       DynIndex.line s i ∈ cft.Q ∧
-       stmt cft (DynIndex.line s i) = some (Stmt.assign v e₀ e₁)) ∨
+       line s i ∈ cft.Q ∧
+       stmt cft (line s i) = some (Stmt.assign v e₀ e₁)) ∨
       (∃ e,
-       DynIndex.line s i ∈ cft.Q ∧
-       stmt cft (DynIndex.line s i) = some (Stmt.returnIf e)))
+       line s i ∈ cft.Q ∧
+       stmt cft (line s i) = some (Stmt.returnIf e)))
 
 -- if s # ∈ Q, then s i ∈ Q and stmt(s i) is a returnIf `if e return` or (s $)# ∈ Q
 def noJunkReturns (cft: CFTrace) : Prop :=
   ∀ s,
-    s # ∈ cft.Q →
+    (s ∘ #) ∈ cft.Q →
       ((∃ i e,
-       DynIndex.line s i ∈ cft.Q ∧
-       stmt cft (DynIndex.line s i) = some (Stmt.returnIf e)) ∨
-      (s $)# ∈ cft.Q)
+       line s i ∈ cft.Q ∧
+       stmt cft (line s i) = some (Stmt.returnIf e)) ∨
+      (s ∘ $) ∘ # ∈ cft.Q)
 
 -- if s $ ∈ Q, then s i ∈ Q and stmt(s i) is a `repeat`
 def noJunkRepeats (cft: CFTrace) : Prop :=
   ∀ s,
-    s $ ∈ cft.Q →
+    s ∘ $ ∈ cft.Q →
       (∃ i,
-       DynIndex.line s i ∈ cft.Q ∧
-       stmt cft (DynIndex.line s i) = some (Stmt.repeat))
+       line s i ∈ cft.Q ∧
+       stmt cft (line s i) = some (Stmt.repeat))
 
 
 def cftClosure (cft: CFTrace) : Prop :=
@@ -169,7 +177,7 @@ def validCFTrace (cft: CFTrace) : Prop :=
   cftClosure cft ∧ cftNoJunk cft
 
 
--- val is an arbitrary variable valuation. Validity based on a quasi execution is defined as prop
+-- val is an arbitrary variable valuation. Validity based on a quasi execution is defined as prop mirroring the paper clauses
 abbrev Valuation :=
   DynIndex → Var → Int → Int
 
@@ -180,12 +188,7 @@ mutual
     | Expr.access x e => val s x (evalExpr cft val s e)
     | Expr.sub e₁ e₂ => evalExpr cft val s e₁ - evalExpr cft val s e₂
     | Expr.cond c => evalCond cft val s c
-    | Expr.fn => match s with
-        | DynIndex.line t _ =>
-          match cft.tar t with
-            | some proc => proc.id
-            | _ => -1             --should not occur in valid execution
-        | _ => -1                 --should not occur in valid execution, except for ε! => Valid programs can't use @fn in prompt!
+
   def evalCond (cft: CFTrace) (val: Valuation) (s: DynIndex): Cond → Int
     | Cond.le e₁ e₂ => if evalExpr cft val s e₁ ≤ evalExpr cft val s e₂ then
         1
@@ -203,7 +206,7 @@ def valCallNoPar (val: Valuation) (q: QuasiExecution) : Prop :=
   ∀ s expr args proc,
     stmt q.cft s = some (Stmt.call expr args) ∧
     q.cft.tar s = some proc →
-      ∀ x, (x ∉ proc.params → val (DynIndex.line s 0) x = q.seed (DynIndex.line s 0) x)
+      ∀ x, (x ∉ proc.params → val (line s 0) x = q.seed (line s 0) x)
 
 -- val(s0) (x) = val(s) (y) if x is param and y is arg for x
 def valCallPar (val: Valuation) (q: QuasiExecution) : Prop :=
@@ -211,7 +214,7 @@ def valCallPar (val: Valuation) (q: QuasiExecution) : Prop :=
     stmt q.cft s = some (Stmt.call expr args) ∧
     q.cft.tar s = some proc ∧
     ∀ x y, (x, y) ∈ (List.zip proc.params args) →
-      (val (DynIndex.line s 0) x =
+      (val (line s 0) x =
        val s (match y with         -- y is of type arg, which can be either ref or var
               | Arg.var v => v
               | Arg.ref v => v))
@@ -219,72 +222,72 @@ def valCallPar (val: Valuation) (q: QuasiExecution) : Prop :=
 -- val(s i+1) (x) (k) = eval (s i, rhs) if stmt (s i) is assignment `x[e] = rhs` with eval(s i, e) = k
 def valAssignHit (val: Valuation) (q: QuasiExecution) : Prop :=
   ∀ s i x k e rhs,
-    stmt q.cft (DynIndex.line s i) = some (Stmt.assign x e rhs) ∧
-    evalExpr q.cft val (DynIndex.line s i) e = k →
-      val (DynIndex.line s (i+1)) x k = evalExpr q.cft val (DynIndex.line s i) rhs
+    stmt q.cft (line s i) = some (Stmt.assign x e rhs) ∧
+    evalExpr q.cft val (line s i) e = k →
+      val (line s (i+1)) x k = evalExpr q.cft val (line s i) rhs
 
 -- val(s i+1) (x) (k) = val(s i) (x) (k) if stmt (s i) is assignment `x[e] = rhs` with eval(s i, e) ≠ k
 def valAssignMiss (val: Valuation) (q: QuasiExecution) : Prop :=
   ∀ s i x e rhs k,
-    stmt q.cft (DynIndex.line s i) = some (Stmt.assign x e rhs) ∧
-    evalExpr q.cft val (DynIndex.line s i) e ≠ k →
-      val (DynIndex.line s (i+1)) x k = val (DynIndex.line s i) x k
+    stmt q.cft (line s i) = some (Stmt.assign x e rhs) ∧
+    evalExpr q.cft val (line s i) e ≠ k →
+      val (line s (i+1)) x k = val (line s i) x k
 
 -- val(s i+1) (x) = val(s i) (x) if stmt (s i) is assignment `y[e] = rhs` with y ≠ x
 def valAssignOther (val: Valuation) (q: QuasiExecution) : Prop :=
   ∀ s i x y e rhs,
-    stmt q.cft (DynIndex.line s i) = some (Stmt.assign y e rhs) ∧
+    stmt q.cft (line s i) = some (Stmt.assign y e rhs) ∧
     y ≠ x →
-      (val (DynIndex.line s (i+1)) x = val (DynIndex.line s i) x)
+      (val (line s (i+1)) x = val (line s i) x)
 
 -- val(s i+1) = val (s i) if stmt (s i) is returnIf `if e return` and s i+1 ∈ Q
 def valNoReturn (val: Valuation) (q: QuasiExecution) : Prop :=
   ∀ s i e,
-    stmt q.cft (DynIndex.line s i) = some (Stmt.returnIf e) ∧
-    (DynIndex.line s (i+1)) ∈ q.cft.Q →
-      val (DynIndex.line s (i+1)) = val (DynIndex.line s i)
+    stmt q.cft (line s i) = some (Stmt.returnIf e) ∧
+    (line s (i+1)) ∈ q.cft.Q →
+      val (line s (i+1)) = val (line s i)
 
 -- val(s #) = val (s i) if stmt (s i) is returnIf `if e return` and s i+1 ∉ Q
 def valReturn (val: Valuation) (q: QuasiExecution) : Prop :=
   ∀ s i e,
-    stmt q.cft (DynIndex.line s i) = some (Stmt.returnIf e) ∧
-    (DynIndex.line s (i+1)) ∉ q.cft.Q →
-      val (s #) = val (DynIndex.line s i)
+    stmt q.cft (line s i) = some (Stmt.returnIf e) ∧
+    (line s (i+1)) ∉ q.cft.Q →
+      val (s ∘ #) = val (line s i)
 
 -- val (s $) = val (s i) if stmt (s i) is `repeat`
 def valRepeat (val: Valuation) (q: QuasiExecution) : Prop :=
   ∀ s i,
-    stmt q.cft (DynIndex.line s i) = some (Stmt.repeat) →
-      val (s $) = val (DynIndex.line s i)
+    stmt q.cft (line s i) = some (Stmt.repeat) →
+      val (s ∘ $) = val (line s i)
 
 -- val (s $ 0) = val (s $)
 def valRepeatEntry (val: Valuation) (q: QuasiExecution) : Prop :=
   ∀ s,
-    s $ ∈ q.cft.Q →
-      val (DynIndex.line (s $) 0) = val (s $)
+    s ∘ $ ∈ q.cft.Q →
+      val (line (s ∘ $) 0) = val (s ∘ $)
 
 
 -- val (s #) = val (s $ #)
 def valRepeatReturn (val: Valuation) (q: QuasiExecution) : Prop :=
   ∀ s,
-    (s $) # ∈ q.cft.Q →
-      val (s #) = val ((s $) #)
+    (s ∘ $) ∘ # ∈ q.cft.Q →
+      val (s ∘ #) = val ((s ∘ $) ∘ #)
 
 -- val (s i+1) (x) = val (s i) (x) if stmtm (s i) is `call expr args` and no args are passed by `ref`
 def valCallReturnByValue (val: Valuation) (q: QuasiExecution) : Prop :=
   ∀ s i expr args proc,
-    stmt q.cft (DynIndex.line s i) = some (Stmt.call expr args) ∧
-    q.cft.tar (DynIndex.line s i) = some proc ∧
+    stmt q.cft (line s i) = some (Stmt.call expr args) ∧
+    q.cft.tar (line s i) = some proc ∧
     ∀ x, Arg.ref x ∉ args →
-      (val (DynIndex.line s (i+1)) x = val (DynIndex.line s i) x)
+      (val (line s (i+1)) x = val (line s i) x)
 
 -- val (s i+1) (x) = val (s i #) (y) if stmt (s i) is `call expr args` and x was passed for param x by `ref`
 def valCallReturnByRef (val: Valuation) (q: QuasiExecution) : Prop :=
   ∀ s i expr args proc,
-    stmt q.cft (DynIndex.line s i) = some (Stmt.call expr args) ∧
-    q.cft.tar (DynIndex.line s i) = some proc ∧
+    stmt q.cft (line s i) = some (Stmt.call expr args) ∧
+    q.cft.tar (line s i) = some proc ∧
     ∀ x y, (y, Arg.ref x) ∈ List.zip proc.params args →
-      (val (DynIndex.line s (i +1)) x = val ((DynIndex.line s i) #) y)
+      (val (line s (i +1)) x = val ((line s i) ∘ #) y)
 
 def validValuation (val: Valuation) (q: QuasiExecution) : Prop :=
   valRoot val q ∧
@@ -304,12 +307,12 @@ def validValuation (val: Valuation) (q: QuasiExecution) : Prop :=
 
 -- constrain quasi executions to obtain executions
 
--- if stmt(s i) is returnIf `if e return` then s i+1 ∈ Q ↔ eval(s i, cond) --TODO: Paper mistake?
+-- if stmt(s i) is returnIf `if e return` then s i+1 ∈ Q ↔ eval(s i, cond)
 def execReturn (val: Valuation) (q: QuasiExecution) : Prop :=
   ∀ s i e,
-    stmt q.cft (DynIndex.line s i) = some (Stmt.returnIf e) →
-      (DynIndex.line s (i+1) ∈ q.cft.Q ↔
-       evalExpr q.cft val (DynIndex.line s i) e = 0)
+    stmt q.cft (line s i) = some (Stmt.returnIf e) →
+      (line s (i+1) ∈ q.cft.Q ↔
+       evalExpr q.cft val (line s i) e = 0)
 
 -- if stmt(s) is `call expr args`, then tar(s) = eval(s, expr)
 def execCallTarget (val: Valuation) (q: QuasiExecution) : Prop :=
@@ -323,7 +326,7 @@ def execCallFn (val: Valuation) (q: QuasiExecution) : Prop :=
   ∀ s expr args proc,
     stmt q.cft s = some (Stmt.call expr args) ∧
     q.cft.tar s = some proc →
-      proc.id = evalExpr q.cft val (DynIndex.line s 0) Expr.fn
+      proc.id = evalExpr q.cft val (line s 0) (Expr.access Var.fn (Expr.const 0))
 
 def validExecution (val: Valuation) (q: QuasiExecution) : Prop :=
   execReturn val q ∧
@@ -342,20 +345,16 @@ structure Execution where
   hExec: validExecution val quasi
 
 
-
 def executionModel (e: Execution) :
   DL.KripkeModel DL.DynIdxSym Cond DynIndex where
   val := λ cond s ↦ s ∈ e.quasi.cft.Q ∧ evalCond e.quasi.cft e.val s cond = 1
-  rel := λ a u ua ↦ u ∈ e.quasi.cft.Q ∧ match a with
-                                        | .line i =>
-                                          ua = DynIndex.line u i ∧
-                                          ua ∈ e.quasi.cft.Q
+  rel := λ a u ua ↦ u ∈ e.quasi.cft.Q ∧ ua ∈ e.quasi.cft.Q ∧ match a with
+                                       | .line i =>
+                                          ua = line u i
                                         | .dollar =>
-                                          ua = u $ ∧
-                                          ua ∈ e.quasi.cft.Q
+                                          ua = u ∘ $
                                         | .hash =>
-                                          ua = u # ∧
-                                          ua ∈ e.quasi.cft.Q
+                                          ua = u ∘ #
 
 
-end Logic.REPEAT
+end Logic.DL
