Logic/Common/DynamicIndex.lean
@@ -1,0 +1,32 @@
+namespace Logic.DL
+
+inductive DynIdxSym where
+  | line : Nat → DynIdxSym
+  | hash : DynIdxSym
+  | dollar : DynIdxSym
+deriving DecidableEq
+
+inductive DynIndex where
+  | root : DynIndex
+  | cons : DynIndex → DynIdxSym → DynIndex
+deriving DecidableEq
+
+def line (ι: DynIndex) (n: Nat) :=
+  DynIndex.cons ι (DynIdxSym.line n)
+
+def dollar (ι: DynIndex) :=
+  DynIndex.cons ι DynIdxSym.dollar
+
+def hash (ι: DynIndex) :=
+  DynIndex.cons ι DynIdxSym.hash
+
+instance : Coe Nat DynIdxSym where
+  coe := DynIdxSym.line
+
+notation "ε" => DynIndex.root
+notation "$" => DynIdxSym.dollar
+notation "#" => DynIdxSym.hash
+notation "ι" => DynIdxSym.line
+infixl:80 "∘" => DynIndex.cons
+
+end Logic.DL
