Logic/DL/Notation.lean
@@ -1,16 +1,20 @@
 import Logic.DL.Syntax
+import Logic.REPEAT.Semantics
+
+
 namespace Logic.DL
 
 /-
 # Remarks
-- This approach is only applicable when using the monomorphic DAForm, which fixes DynamicIndices and Atoms as DLForm Types.
+- This approach is only applicable when using the monomorphic DAForm, which fixes DynamicIndices and Cond as DLForm Types.
 - In order to avoid confusion with Leans inbuilt notation for Props, the following logical connectives have to be chosen slightly different than usual textbook:
   • `⋎` for DL "or"
   • `⋏` for DL "and"
   • `∼` for DL "not"
 -/
 
-
+--formulas
+abbrev DAForm := DLForm DynIdxSym Cond
 -- relevant coercions
 instance: Coe DynIdxSym (Relation DynIdxSym) where
   coe α := Relation.relAtom α
@@ -21,16 +25,13 @@ instance: OfNat DynIdxSym n where
 instance: OfNat (Relation DynIdxSym) n where
   ofNat := Relation.relAtom (DynIdxSym.line n)
 
-instance: Coe String (DLForm DynIdxSym Atoms) where
-  coe p := DLForm.atom (Atoms.name p)
+instance: Coe String Expr where
+  coe s := Expr.var (Var.name s)
 
-instance: Coe String Atoms where
-  coe p := Atoms.name p
+instance: Coe Cond DAForm where
+  coe c := DLForm.atom c
 
 --basic notations
-notation "$" => DynIdxSym.dollar
-notation "#" => DynIdxSym.hash
-
 notation "∅" => Relation.emptyset
 notation "•" => Relation.wild
 
@@ -38,12 +39,11 @@ notation "⊥" => DLForm.falsum
 
 
 --relation operators
-notation:max α "*" => Relation.iter (α: Relation DynIdxSym)
+notation:100 α "*" => Relation.iter (α: Relation DynIdxSym)
 notation:80 α:81 β:80 => Relation.comp (α: Relation DynIdxSym) (β: Relation DynIdxSym)
 notation:70 α:71 " ∪ " β:70 => Relation.alt (α: Relation DynIdxSym) (β: Relation DynIdxSym)
 
---formulas
-abbrev DAForm := DLForm DynIdxSym Atoms
+
 
 
 notation:90 "⟨" α "⟩" φ => DLForm.diamond (α: Relation DynIdxSym) (φ: DAForm)
@@ -54,16 +54,14 @@ notation:60 φ:61 " ⋎ " ψ:60 => disj (φ: DAForm) (ψ: DAForm)
 notation:50 φ:51 " → " ψ:50 => DLForm.imp (φ: DAForm) (ψ: DAForm)
 
 
+infix:110 "=ₑ" => Expr.Cond.eq
+infix:110 "<ₑ" => Cond.le
+
 #check 0 1 2 3 #
-#check [(0 1 * ∪ 1)*] "p"
+#check [(0 1 * ∪ 1)*]
 #check 0 ∪ 1 * ∪ #
-#check ∼ ⟨0 $⟩   ∼ "p" ⋎ "q" --
-#check ∼⟨0 #⟩ (∼ "p") ⋎ "q"
-#check "p" ⋎ "q" ⋏ "p"
-#check "p" ⋏ "q" ⋎ "p"
-#check "p" ⋏ ⊥ ⋎ "p"
-#check "p" ⋎ "p" ⋎ "p" ⋏ "q" ⋎ "q"
-#check "p" → "q"
+#check ⟨0 $⟩ ("p" =ₑ "q")
+#check ∼⟨0 #⟩ (∼ "p" <ₑ "q") ⋎ "q" <ₑ "p"
 #check ⊥
 #check #
 #check ∅
